Use new [aux_unchanged_payload] lemmas to prove for insertion at head and tail

ind/DoublyLinkedList.fst
@@ -1424,9 +1424,9 @@ let dll_insert_at_head (#t:Type) (d:dll t) (n:pointer (node t)) :
     n <|= h;
     let h1 = ST.get () in
     //
-    let rec unchanged_payload nl : Lemma (unchanged_node_vals h0 h1 nl) =
-      if (length nl = 0) then () else unchanged_payload (tl nl) in
-    unchanged_payload (reveal d.nodes);
+    aux_unchanged_payload h0 h0' n (reveal d.nodes);
+    aux_unchanged_payload h0' h1 h (reveal d.nodes);
+    aux_unchanged_payload_transitive h0 h0' h1 (reveal d.nodes);
     //
     let Frag1 p1 = tot_dll_to_fragment h0 d in
     let p = tot_node_to_piece h0 n in
@@ -1491,17 +1491,19 @@ let dll_insert_at_tail (#t:Type) (d:dll t) (n:pointer (node t)) :
     t =|> n;
     let h1 = ST.get () in
     //
-    let rec unchanged_payload nl : Lemma (unchanged_node_vals h0 h1 nl) =
-      if (length nl = 0) then () else unchanged_payload (tl nl) in
-    unchanged_payload (reveal d.nodes);
-    //
     let Frag1 p1 = tot_dll_to_fragment h0 d in
     let p = tot_node_to_piece h0 n in
     let f' = Frag2 p1 p in
     piece_remains_valid h0 h0' (Mod.loc_buffer n) p1;
     piece_remains_valid_f h0' h1 p1;
     let y = tot_defragmentable_fragment_to_dll h1 f' in
-    unchanged_payload (reveal y.nodes);
+    lemma_unsnoc_is_last (reveal y.nodes);
+    lemma_snoc_unsnoc (reveal d.nodes, n);
+    lemma_unsnoc_index (reveal y.nodes) (length (reveal y.nodes) - 2);
+    lemma_unsnoc_length (reveal y.nodes);
+    aux_unchanged_payload h0 h0' n (reveal y.nodes);
+    aux_unchanged_payload h0' h1 t (reveal y.nodes);
+    aux_unchanged_payload_transitive h0 h0' h1 (reveal y.nodes);
     y
   )
 
